putting hand-edited extraction folder in parallel

proofs/fstar/extraction-edited/Libcrux.Kem.Kyber.Ntt.fst
@@ -31,7 +31,8 @@ let ntt_multiply_binomials (a0, a1: (i32 & i32)) (b0, b1: (i32 & i32)) (zeta: i3
   <:
   (i32 & i32)
 
-let invert_ntt_montgomery (v_K: usize) (re: Libcrux.Kem.Kyber.Arithmetic.t_PolynomialRingElement) =
+let invert_ntt_montgomery (v_K: usize) (re: Libcrux.Kem.Kyber.Arithmetic.t_PolynomialRingElement)
+    : Libcrux.Kem.Kyber.Arithmetic.t_PolynomialRingElement =
   let _:Prims.unit = () <: Prims.unit in
   let zeta_i:usize = Libcrux.Kem.Kyber.Constants.v_COEFFICIENTS_IN_RING_ELEMENT /! sz 2 in
   let step:usize = sz 1 <<! 1l in
@@ -581,7 +582,55 @@ let invert_ntt_montgomery (v_K: usize) (re: Libcrux.Kem.Kyber.Arithmetic.t_Polyn
   in
   re
 
-let ntt_binomially_sampled_ring_element (re: Libcrux.Kem.Kyber.Arithmetic.t_PolynomialRingElement) =
+let ntt_binomially_sampled_ring_element (re: Libcrux.Kem.Kyber.Arithmetic.t_PolynomialRingElement)
+    : Prims.Pure Libcrux.Kem.Kyber.Arithmetic.t_PolynomialRingElement
+      (requires
+        Hax_lib.v_forall (fun i ->
+              let i:usize = i in
+              Hax_lib.implies (i <.
+                  (Core.Slice.impl__len (Rust_primitives.unsize re
+                            .Libcrux.Kem.Kyber.Arithmetic.f_coefficients
+                        <:
+                        t_Slice i32)
+                    <:
+                    usize)
+                  <:
+                  bool)
+                ((Core.Num.impl__i32__abs (re.Libcrux.Kem.Kyber.Arithmetic.f_coefficients.[ i ]
+                        <:
+                        i32)
+                    <:
+                    i32) <=.
+                  3l
+                  <:
+                  bool)
+              <:
+              bool))
+      (ensures
+        fun result ->
+          let result:Libcrux.Kem.Kyber.Arithmetic.t_PolynomialRingElement = result in
+          Hax_lib.v_forall (fun i ->
+                let i:usize = i in
+                Hax_lib.implies (i <.
+                    (Core.Slice.impl__len (Rust_primitives.unsize result
+                              .Libcrux.Kem.Kyber.Arithmetic.f_coefficients
+                          <:
+                          t_Slice i32)
+                      <:
+                      usize)
+                    <:
+                    bool)
+                  ((Core.Num.impl__i32__abs (result.Libcrux.Kem.Kyber.Arithmetic.f_coefficients.[ i
+                          ]
+                          <:
+                          i32)
+                      <:
+                      i32) <.
+                    Libcrux.Kem.Kyber.Constants.v_FIELD_MODULUS
+                    <:
+                    bool)
+                <:
+                bool)) =
   let _:Prims.unit = () <: Prims.unit in
   let zeta_i:usize = sz 0 in
   let zeta_i:usize = zeta_i +! sz 1 in
@@ -1067,7 +1116,51 @@ let ntt_binomially_sampled_ring_element (re: Libcrux.Kem.Kyber.Arithmetic.t_Poly
   in
   re
 
-let ntt_multiply (lhs rhs: Libcrux.Kem.Kyber.Arithmetic.t_PolynomialRingElement) =
+let ntt_multiply (lhs rhs: Libcrux.Kem.Kyber.Arithmetic.t_PolynomialRingElement)
+    : Prims.Pure Libcrux.Kem.Kyber.Arithmetic.t_PolynomialRingElement
+      (requires
+        Hax_lib.v_forall (fun i ->
+              let i:usize = i in
+              Hax_lib.implies (i <. Libcrux.Kem.Kyber.Constants.v_COEFFICIENTS_IN_RING_ELEMENT
+                  <:
+                  bool)
+                (((lhs.Libcrux.Kem.Kyber.Arithmetic.f_coefficients.[ i ] <: i32) >=. 0l <: bool) &&
+                  ((lhs.Libcrux.Kem.Kyber.Arithmetic.f_coefficients.[ i ] <: i32) <. 4096l <: bool) &&
+                  ((Core.Num.impl__i32__abs (rhs.Libcrux.Kem.Kyber.Arithmetic.f_coefficients.[ i ]
+                          <:
+                          i32)
+                      <:
+                      i32) <=.
+                    Libcrux.Kem.Kyber.Constants.v_FIELD_MODULUS
+                    <:
+                    bool))
+              <:
+              bool))
+      (ensures
+        fun result ->
+          let result:Libcrux.Kem.Kyber.Arithmetic.t_PolynomialRingElement = result in
+          Hax_lib.v_forall (fun i ->
+                let i:usize = i in
+                Hax_lib.implies (i <.
+                    (Core.Slice.impl__len (Rust_primitives.unsize result
+                              .Libcrux.Kem.Kyber.Arithmetic.f_coefficients
+                          <:
+                          t_Slice i32)
+                      <:
+                      usize)
+                    <:
+                    bool)
+                  ((Core.Num.impl__i32__abs (result.Libcrux.Kem.Kyber.Arithmetic.f_coefficients.[ i
+                          ]
+                          <:
+                          i32)
+                      <:
+                      i32) <=.
+                    Libcrux.Kem.Kyber.Constants.v_FIELD_MODULUS
+                    <:
+                    bool)
+                <:
+                bool)) =
   let _:Prims.unit = () <: Prims.unit in
   let out:Libcrux.Kem.Kyber.Arithmetic.t_PolynomialRingElement =
     Libcrux.Kem.Kyber.Arithmetic.impl__PolynomialRingElement__ZERO
@@ -1214,7 +1307,7 @@ let ntt_vector_u
                     usize)
                   <:
                   bool)
-                (fun _ -> (Core.Num.impl__i32__abs (re.Libcrux.Kem.Kyber.Arithmetic.f_coefficients.[ i ]
+                ((Core.Num.impl__i32__abs (re.Libcrux.Kem.Kyber.Arithmetic.f_coefficients.[ i ]
                         <:
                         i32)
                     <:
@@ -1238,7 +1331,7 @@ let ntt_vector_u
                       usize)
                     <:
                     bool)
-                  (fun _ -> (Core.Num.impl__i32__abs (result.Libcrux.Kem.Kyber.Arithmetic.f_coefficients.[ i
+                  ((Core.Num.impl__i32__abs (result.Libcrux.Kem.Kyber.Arithmetic.f_coefficients.[ i
                           ]
                           <:
                           i32)
