proofs/fstar/extraction-snapshot/Libcrux.Kem.Kyber.Ntt.fst
@@ -23,6 +23,7 @@ let v_ZETAS_TIMES_MONTGOMERY_R: t_Array i32 (sz 128) =
   Rust_primitives.Hax.array_of_list list
 
 let ntt_multiply_binomials (a0, a1: (i32 & i32)) (b0, b1: (i32 & i32)) (zeta: i32) : (i32 & i32) =
+  admit(); // Needs preconditions on ranges of all inputs
   Libcrux.Kem.Kyber.Arithmetic.montgomery_reduce ((a0 *! b0 <: i32) +!
       ((Libcrux.Kem.Kyber.Arithmetic.montgomery_reduce (a1 *! b1 <: i32) <: i32) *! zeta <: i32)
       <:
@@ -35,6 +36,7 @@ let invert_ntt_montgomery (v_K: usize) (re: Libcrux.Kem.Kyber.Arithmetic.t_Polyn
   let _:Prims.unit = () <: Prims.unit in
   let zeta_i:usize = Libcrux.Kem.Kyber.Constants.v_COEFFICIENTS_IN_RING_ELEMENT /! sz 2 in
   let step:usize = sz 1 <<! 1l in
+  admit(); // Needs many preconditions and is too big, break it up.
   let re, zeta_i:(Libcrux.Kem.Kyber.Arithmetic.t_PolynomialRingElement & usize) =
     Core.Iter.Traits.Iterator.f_fold (Core.Iter.Traits.Collect.f_into_iter ({
               Core.Ops.Range.f_start = sz 0;
@@ -47,6 +49,7 @@ let invert_ntt_montgomery (v_K: usize) (re: Libcrux.Kem.Kyber.Arithmetic.t_Polyn
       (re, zeta_i <: (Libcrux.Kem.Kyber.Arithmetic.t_PolynomialRingElement & usize))
       (fun temp_0_ round ->
           let re, zeta_i:(Libcrux.Kem.Kyber.Arithmetic.t_PolynomialRingElement & usize) = temp_0_ in
+          assume (zeta_i >. sz 1);
           let round:usize = round in
           let zeta_i:usize = zeta_i -! sz 1 in
           let offset:usize = (round *! step <: usize) *! sz 2 in
@@ -598,10 +601,12 @@ let ntt_binomially_sampled_ring_element (re: Libcrux.Kem.Kyber.Arithmetic.t_Poly
       (fun re j ->
           let re:Libcrux.Kem.Kyber.Arithmetic.t_PolynomialRingElement = re in
           let j:usize = j in
+          assume (range (v #i32_inttype re.f_coefficients.[j +! sz 128] * (-1600)) i32_inttype);
           let t:i32 =
             (re.Libcrux.Kem.Kyber.Arithmetic.f_coefficients.[ j +! sz 128 <: usize ] <: i32) *!
             (-1600l)
           in
+          assume (range (v #i32_inttype re.f_coefficients.[j] - v t) i32_inttype);
           let re:Libcrux.Kem.Kyber.Arithmetic.t_PolynomialRingElement =
             {
               re with
@@ -615,6 +620,7 @@ let ntt_binomially_sampled_ring_element (re: Libcrux.Kem.Kyber.Arithmetic.t_Poly
             <:
             Libcrux.Kem.Kyber.Arithmetic.t_PolynomialRingElement
           in
+          assume (range (v #i32_inttype re.f_coefficients.[j] + v t) i32_inttype);
           let re:Libcrux.Kem.Kyber.Arithmetic.t_PolynomialRingElement =
             {
               re with
@@ -632,6 +638,7 @@ let ntt_binomially_sampled_ring_element (re: Libcrux.Kem.Kyber.Arithmetic.t_Poly
   in
   let _:Prims.unit = () <: Prims.unit in
   let step:usize = sz 1 <<! 6l in
+  admit(); // Too big, break up.
   let re, zeta_i:(Libcrux.Kem.Kyber.Arithmetic.t_PolynomialRingElement & usize) =
     Core.Iter.Traits.Iterator.f_fold (Core.Iter.Traits.Collect.f_into_iter ({
               Core.Ops.Range.f_start = sz 0;
@@ -644,6 +651,7 @@ let ntt_binomially_sampled_ring_element (re: Libcrux.Kem.Kyber.Arithmetic.t_Poly
       (re, zeta_i <: (Libcrux.Kem.Kyber.Arithmetic.t_PolynomialRingElement & usize))
       (fun temp_0_ round ->
           let re, zeta_i:(Libcrux.Kem.Kyber.Arithmetic.t_PolynomialRingElement & usize) = temp_0_ in
+          assume (v zeta_i < maxint usize_inttype);
           let round:usize = round in
           let zeta_i:usize = zeta_i +! sz 1 in
           let offset:usize = (round *! step <: usize) *! sz 2 in
@@ -1087,6 +1095,7 @@ let ntt_multiply (lhs rhs: Libcrux.Kem.Kyber.Arithmetic.t_PolynomialRingElement)
       (fun out i ->
           let out:Libcrux.Kem.Kyber.Arithmetic.t_PolynomialRingElement = out in
           let i:usize = i in
+          assume (v i * 4 + 4 <= 256);
           let product:(i32 & i32) =
             ntt_multiply_binomials ((lhs.Libcrux.Kem.Kyber.Arithmetic.f_coefficients.[ sz 4 *! i
                     <:
